refinement to tail-rec, started general pattern for IMP- to IMP--

Cook_Levin/IMP-_To_SAS+/IMP--_To_SAS++/IMP_Minus_Minus_Subprograms_Nat.thy
@@ -6,19 +6,61 @@ begin
 fun map_all_subprograms:: "nat \<Rightarrow> nat \<Rightarrow> nat" where 
 "map_all_subprograms c n = (if n =0 then 0 else (2## (hd_nat n) ## (nth_nat (Suc (Suc 0)) c ) ## 0) ## map_all_subprograms c (tl_nat n) )"
 
+fun map_all_subprograms_acc:: "nat \<Rightarrow> nat \<Rightarrow> nat \<Rightarrow> nat" where 
+"map_all_subprograms_acc c acc n = (if n =0 then acc else map_all_subprograms_acc c ((2## (hd_nat n) ## (nth_nat (Suc (Suc 0)) c ) ## 0) ## acc ) (tl_nat n) )"
+
+lemma map_all_subprograms_induct:
+"map_all_subprograms_acc c acc n = map_acc (\<lambda>c'. 2## c' ## (nth_nat (Suc (Suc 0)) c ) ## 0) acc n"
+  apply(induct c acc n rule: map_all_subprograms_acc.induct)
+  apply(auto)
+  done
+
+definition map_all_subprograms_tail :: "nat \<Rightarrow> nat \<Rightarrow> nat" where 
+"map_all_subprograms_tail c n = reverse_nat (map_all_subprograms_acc c 0 n)"
+
 lemma submap_all_subprograms:
   "map_all_subprograms c n = map_nat (\<lambda>c'. 2## c' ## (nth_nat (Suc (Suc 0)) c ) ## 0) n"
   apply (induct c n rule: map_all_subprograms.induct)
   apply auto
   done
 
+lemma subtail_map_all_subprograms:
+"map_all_subprograms_tail c n = map_all_subprograms c n"
+  using submap_all_subprograms map_all_subprograms_tail_def  map_all_subprograms_induct[of c 0 n]
+  subtail_map by presburger
+
+
+
 fun map_all_subprograms2:: "nat \<Rightarrow> nat \<Rightarrow> nat" where 
 "map_all_subprograms2 c n = (if n =0 then 0 else ( 2## (hd_nat n) ## c ## 0) ## map_all_subprograms2 c (tl_nat n) )"
+
+
 lemma submap_all_subprograms2:
 "map_all_subprograms2 c n = map_nat (\<lambda>x. 2## x ## c ## 0) n"
   apply (induct c n rule: map_all_subprograms2.induct)
   apply auto
   done
+
+fun map_all_subprograms2_acc:: "nat \<Rightarrow> nat \<Rightarrow> nat \<Rightarrow> nat" where 
+"map_all_subprograms2_acc  c acc n = (if n =0 then acc else 
+map_all_subprograms2_acc c (( 2## (hd_nat n) ## c ## 0) ## acc) (tl_nat n) )"
+
+lemma  map_all_subprograms2_induct:
+" map_all_subprograms2_acc c acc n = map_acc  (\<lambda>x. 2## x ## c ## 0) acc n"
+  apply(induct c acc n rule:map_all_subprograms2_acc.induct)
+  apply auto
+  done
+
+definition map_all_subprograms2_tail :: "nat \<Rightarrow> nat \<Rightarrow> nat" where 
+"map_all_subprograms2_tail c n = reverse_nat (map_all_subprograms2_acc c 0 n)"
+
+lemma subtail_map_all_subprograms2:
+"map_all_subprograms2_tail c n = map_all_subprograms2 c n"
+  using submap_all_subprograms2 map_all_subprograms2_tail_def  map_all_subprograms2_induct[of c 0 n]
+  subtail_map by presburger
+
+
+
 
 declare nth_nat.simps[simp del]
 fun all_subprograms_nat :: "nat \<Rightarrow> nat" where
@@ -69,6 +111,10 @@ fun all_variables_nat :: "nat \<Rightarrow>nat" where
 if hd_nat n = 1 then (nth_nat (Suc 0) n) ## 0 else
 nth_nat (Suc 0) n )"
 
+definition all_variables_tail where "all_variables_tail = all_variables_nat"
+
+lemma subtail_all_variables : "all_variables_tail = all_variables_nat" using  all_variables_tail_def by meson
+
 lemma sub_all_variables: "all_variables_nat (comm_encode c) = vname_list_encode (all_variables c)"
   apply (cases c)
       apply (auto simp only:all_variables_nat.simps sub_hd comm_encode.simps head.simps 
@@ -78,11 +124,29 @@ lemma sub_all_variables: "all_variables_nat (comm_encode c) = vname_list_encode 
 
 fun map_all_variables:: "nat \<Rightarrow> nat" where 
 "map_all_variables n = (if n =0 then 0 else (all_variables_nat (hd_nat n)) ## map_all_variables (tl_nat n) )"
+
+fun map_all_variables_acc :: "nat \<Rightarrow> nat \<Rightarrow> nat" where 
+"map_all_variables_acc acc n = (if n =0 then acc else map_all_variables_acc ((all_variables_tail (hd_nat n)) ## acc) (tl_nat n) )"
+
 lemma submap_all_variables:
 "map_all_variables n = map_nat all_variables_nat n"
   apply (induct n rule:map_all_variables.induct)
   apply auto
   done
+lemma  map_all_variables_induct:
+" map_all_variables_acc acc n = map_acc all_variables_nat acc n"
+  apply(induct acc n rule: map_all_variables_acc.induct)
+  apply (auto simp add: subtail_all_variables )
+  done
+
+definition map_all_variables_tail :: "nat \<Rightarrow> nat" where 
+" map_all_variables_tail n = reverse_nat (map_all_variables_acc 0 n)"
+
+lemma subtail_map_all_variables:
+" map_all_variables_tail n  =  map_all_variables n "
+  using map_all_variables_tail_def  map_all_variables_induct[of 0 n]
+  submap_all_variables subtail_map by presburger
+
 
 definition enumerate_variables_nat :: "nat \<Rightarrow> nat" where
 "enumerate_variables_nat c =
