Cook_Levin/IMP-_To_SAS+/IMP-_To_IMP--/Binary_Operations_Nat.thy
@@ -33,9 +33,10 @@ lemma com_list_to_seq_rev: "com_list_to_seq_nat (append_nat ys xs) =
 
 definition  com_list_to_seq_tail :: "nat \<Rightarrow> nat" where 
 "com_list_to_seq_tail ys = com_list_to_seq_acc  (0##0) (reverse_nat ys) "
+
 lemma subtail_com_list_to_seq: "com_list_to_seq_nat ys=
-       com_list_to_seq_acc  (0##0) (reverse_nat ys)"
-  using  com_list_to_seq_rev[of ys 0]  append_nat_0 
+      com_list_to_seq_tail ys"
+  using  com_list_to_seq_rev[of ys 0]  append_nat_0  com_list_to_seq_tail_def 
   by(auto)
 
 
@@ -155,6 +156,28 @@ fun copy_const_to_operand_nat :: "nat \<Rightarrow> nat \<Rightarrow> nat \<Righ
 2 ## (1 ## (operand_bit_to_var_nat (prod_encode (op,i-1))) ## (nth_bit_nat x (i-1)) ## 0) ## (copy_const_to_operand_nat (i-1) op x ) ## 0
 )"
 
+fun copy_const_to_operand_acc :: "nat \<Rightarrow> nat \<Rightarrow> nat \<Rightarrow> nat \<Rightarrow> nat \<Rightarrow> nat" where 
+"copy_const_to_operand_acc acc diff i op x = (if diff =0 then acc  else copy_const_to_operand_acc
+(2 ## (1 ## (operand_bit_to_var_tail (prod_encode (op,i-diff))) ## (nth_bit_tail x (i-diff)) ## 0) ## acc ## 0
+) (diff-1) i op x )"
+
+lemma copy_const_to_operand_induct:
+"diff\<le>i \<Longrightarrow>copy_const_to_operand_acc (copy_const_to_operand_nat (i-diff) op x) diff i op x =
+copy_const_to_operand_nat i op x"
+  apply(induct diff)
+   apply(auto simp add: subtail_operand_bit_to_var subtail_nth_bit)
+  done
+
+definition copy_const_to_operand_tail :: "nat \<Rightarrow> nat \<Rightarrow> nat \<Rightarrow> nat" where 
+"copy_const_to_operand_tail i op x = copy_const_to_operand_acc (0##0) i i op x"
+
+lemma subtail_copy_const_to_operand:
+"copy_const_to_operand_tail i op x = 
+copy_const_to_operand_nat i op x "
+  using copy_const_to_operand_induct [of i i op x]
+  apply(auto simp add:copy_const_to_operand_tail_def)
+  done
+
 lemma sub_copy_const_to_operand:
  "copy_const_to_operand_nat i (encode_char op) x = comm_encode (copy_const_to_operand i op x)  "
  apply (induct i)
@@ -171,6 +194,14 @@ definition copy_atom_to_operand_nat:: "nat \<Rightarrow> nat \<Rightarrow> nat \
 "copy_atom_to_operand_nat n op a = ( if fst_nat a = 0 then  copy_var_to_operand_nat n op (snd_nat a)
  else copy_const_to_operand_nat n op (snd_nat a))"
 
+definition copy_atom_to_operand_tail:: "nat \<Rightarrow> nat \<Rightarrow> nat \<Rightarrow> nat" where 
+"copy_atom_to_operand_tail n op a = ( if fst_nat a = 0 then  copy_var_to_operand_tail n op (snd_nat a)
+ else copy_const_to_operand_nat n op (snd_nat a))"
+
+lemma subtail_copy_atom_to_operand: "copy_atom_to_operand_tail n op a = copy_atom_to_operand_nat n op a"
+  apply (simp only: copy_atom_to_operand_tail_def copy_atom_to_operand_nat_def
+subtail_copy_var_to_operand  ) done
+
 lemma sub_copy_atom_to_operand: 
 "copy_atom_to_operand_nat n (encode_char op) (atomExp_encode a) = comm_encode (copy_atom_to_operand n op a)"
   apply (auto simp only:copy_atom_to_operand_nat_def atomExp_encode.simps sub_fst sub_snd fst_def snd_def
@@ -185,6 +216,19 @@ definition assign_var_carry_nat::
 "assign_var_carry_nat i v a b c = 
 2 ## (1 ## (var_bit_to_var_nat(prod_encode (v, i))) ##
 (if a + b + c = 1 \<or> a + b + c = 3 then 1 else 0) ## 0 ) ## (1##(vname_encode ''carry'')## (if a + b + c \<ge> 2 then 1 else 0) ## 0) ## 0 "
+
+definition assign_var_carry_tail :: "nat \<Rightarrow> nat \<Rightarrow> nat \<Rightarrow> nat \<Rightarrow> nat \<Rightarrow> nat"  where 
+"assign_var_carry_tail i v a b c = 
+2 ## (1 ## (var_bit_to_var_tail(prod_encode (v, i))) ##
+(if a + b + c = 1 \<or> a + b + c = 3 then 1 else 0) ## 0 ) ## (1##(vname_encode ''carry'')## (if a + b + c \<ge> 2 then 1 else 0) ## 0) ## 0 "
+
+
+lemma subtail_assign_var_carry: 
+"assign_var_carry_tail  i v a b c = assign_var_carry_nat  i v a b c"
+  apply (auto simp  only: assign_var_carry_tail_def assign_var_carry_nat_def 
+        subtail_var_bit_to_var)
+  done
+
 
 lemma sub_assign_var_carry: 
 "assign_var_carry_nat i (vname_encode v) a b c = comm_encode(assign_var_carry i v a b c)"
@@ -204,6 +248,22 @@ definition full_adder_nat:: "nat \<Rightarrow> nat \<Rightarrow> nat" where
 ## 0
  )"
 
+definition full_adder_tail ::  "nat \<Rightarrow> nat \<Rightarrow> nat"  where 
+"full_adder_tail i v  = (let assign = assign_var_carry_tail i v; op_a = operand_bit_to_var_tail (prod_encode(encode_char(CHR ''a''), i));
+  op_b = operand_bit_to_var_tail (prod_encode(encode_char (CHR ''b''), i)) in 
+3##(op_a ## 0) ##(3##((vname_encode ''carry'') ## 0)## (3 ## (op_b ## 0) ## (assign 1 1 1) ## ( assign 1 1 0) ## 0)##(
+                                                       (3 ## (op_b ## 0) ## (assign 1 0 1) ## ( assign 1 0 0) ## 0))##0)
+               ##(3##((vname_encode ''carry'') ## 0)## (3 ## (op_b ## 0) ## (assign 0 1 1) ## ( assign 0 1 0) ## 0)##(
+                                                       (3 ## (op_b ## 0) ## (assign 0 0 1) ## ( assign 0 0 0) ## 0))##0)
+## 0
+ )"
+
+
+lemma subtail_full_adder: "full_adder_tail i v = full_adder_nat i v" 
+  apply(auto simp only: Let_def full_adder_tail_def 
+          full_adder_nat_def subtail_assign_var_carry subtail_operand_bit_to_var )
+  done
+
 lemma sub_full_adder: "full_adder_nat i (vname_encode v) = comm_encode (full_adder i v)"
   apply (auto simp only:full_adder_nat_def sub_assign_var_carry
  vname_list_encode_def cons0 sub_cons sub_operand_bit_to_var full_adder_def comm_encode.simps
@@ -214,19 +274,72 @@ lemma sub_full_adder: "full_adder_nat i (vname_encode v) = comm_encode (full_add
 fun map_adder :: "nat \<Rightarrow> nat \<Rightarrow> nat" where 
 "map_adder v n = (if n =0 then 0 else (full_adder_nat (hd_nat n) v) ## map_adder v (tl_nat n))"
 
+fun map_adder_acc :: "nat \<Rightarrow> nat \<Rightarrow> nat \<Rightarrow> nat" where 
+"map_adder_acc acc v n = (if n =0 then acc else map_adder_acc ((full_adder_tail (hd_nat n) v)##acc)
+    v (tl_nat n)) "
+
 lemma sub_map_adder:
   "map_adder v n = map_nat (\<lambda>i. full_adder_nat i v) n"
   apply (induct v n rule:map_adder.induct)
   apply (subst map_adder.simps)
   apply auto
   done
- 
+
+lemma map_adder_append:
+"map_adder v (append_nat xs ys) = append_nat (map_adder v xs) (map_adder v ys)"
+proof -
+  obtain xs' ys' where "xs= list_encode xs'" "ys = list_encode ys'"
+    by (metis list_decode_inverse)
+  thus ?thesis apply (auto simp add:sub_append sub_map_adder sub_map simp del:map_adder.simps 
+map_nat.simps) done
+qed
+
+lemma map_adder_induct: "
+reverse_nat (map_adder v (append_nat xs ys)) = 
+map_adder_acc (reverse_nat (map_adder v xs)) v ys
+  "
+  apply(induct ys arbitrary:xs rule:length_nat.induct)
+   apply(auto simp add: append_nat_0 append_nat_Suc  simp del: map_adder.simps map_adder_acc.simps)
+   apply simp
+  apply(subst (2) map_adder_acc.simps)
+  apply(auto simp add: map_adder_append 
+          reverse_append_nat subtail_full_adder  simp del: map_adder.simps map_adder_acc.simps)
+  apply(subst map_adder.simps)
+ apply(auto simp add:cons_Nil simp del:list_encode.simps map_adder.simps map_adder_acc.simps)
+  apply(auto simp add:cons0 sub_hd sub_tl 
+              simp del:list_encode.simps map_adder.simps map_adder_acc.simps)
+   apply(auto simp add: reverse_cons_nat 
+              simp del: map_adder.simps map_adder_acc.simps)  
+      apply(subst map_adder.simps)
+    apply(auto simp add: reverse_nat_0 append_singleton_nat
+              simp del: map_adder.simps map_adder_acc.simps)  
+  done
+
+definition map_adder_tail  where 
+"map_adder_tail v n = reverse_nat (map_adder_acc 0 v n) "
+
+lemma subtail_map_adder : 
+"map_adder_tail v n = map_adder v n"
+  using map_adder_induct[of v 0 n]  append_nat_0
+  apply (auto simp add: map_adder_tail_def simp  del: map_adder.simps map_adder_acc.simps)
+  using rev_rev_nat 
+  by (metis map_adder.simps reverse_nat_0)
+
+
 definition adder_nat:: "nat \<Rightarrow> nat  \<Rightarrow> nat" where
 "adder_nat n v = 2 ## (com_list_to_seq_nat (map_adder v(list_less_nat n) )) ## (
 1## (vname_encode ''carry'') ## 0 ## 0
 ) ## 0"
 
-thm "comp_apply"
+definition adder_tail:: "nat \<Rightarrow> nat  \<Rightarrow> nat"  
+  where "adder_tail n v = 2 ## (com_list_to_seq_tail (map_adder_tail v(list_less_tail n) )) ## (
+1## (vname_encode ''carry'') ## 0 ## 0
+) ## 0"
+lemma subtail_adder: "adder_tail n v =adder_nat n v" 
+  apply(auto simp only: adder_tail_def adder_nat_def subtail_com_list_to_seq subtail_map_adder
+          subtail_list_less)
+  done
+
 
   
 lemma sub_adder: "adder_nat n (vname_encode v) = comm_encode (adder n v)"
@@ -246,6 +359,23 @@ definition binary_adder_nat:: "nat \<Rightarrow> nat \<Rightarrow>nat\<Rightarro
 )##0
 )##0"
 
+definition binary_adder_tail:: "nat \<Rightarrow> nat \<Rightarrow>nat\<Rightarrow> nat \<Rightarrow> nat" where
+"binary_adder_tail n v a b = 2##(
+    copy_atom_to_operand_tail n (encode_char(CHR ''a'')) a)##(
+2##( copy_atom_to_operand_tail n (encode_char(CHR ''b'')) b)##(
+2##( adder_tail n v)##(
+2##(copy_atom_to_operand_tail n (encode_char(CHR ''a'')) (prod_encode(1,0)))##(
+  copy_atom_to_operand_tail n (encode_char(CHR ''b'')) (prod_encode(1,0)))##0 
+)##0
+)##0
+)##0"
+
+lemma subtail_binary_adder:
+"binary_adder_tail n v a b  = binary_adder_nat n v a b "
+  apply(auto simp only: binary_adder_nat_def binary_adder_tail_def subtail_copy_atom_to_operand
+        subtail_adder)
+  done
+
 lemma sub_binary_adder:
  "binary_adder_nat n (vname_encode v) (atomExp_encode a) (atomExp_encode b) =
     comm_encode (binary_adder n v a b)"
@@ -261,6 +391,21 @@ definition assign_var_carry_sub_nat::
 (if b + c = 0 \<or> b + c = 2 then (if a = 1 then 1 else 0)
     else (if b + c = 1 \<and> a = 0 then 1 else 0))  ## 0 ) ## 
 (1##(vname_encode ''carry'')## (if a < b + c then 1 else 0) ## 0) ## 0 "
+
+definition assign_var_carry_sub_tail:: 
+  "nat \<Rightarrow> nat \<Rightarrow> nat \<Rightarrow> nat \<Rightarrow> nat \<Rightarrow> nat" where
+"assign_var_carry_sub_tail i v a b c = 
+2 ## (1 ## (var_bit_to_var_tail (prod_encode (v, i))) ##
+(if b + c = 0 \<or> b + c = 2 then (if a = 1 then 1 else 0)
+    else (if b + c = 1 \<and> a = 0 then 1 else 0))  ## 0 ) ## 
+(1##(vname_encode ''carry'')## (if a < b + c then 1 else 0) ## 0) ## 0 "
+
+lemma subtail_assign_var_carry_sub:
+"assign_var_carry_sub_tail i v a b c = assign_var_carry_sub_nat i v a b c"
+  apply(auto simp only: assign_var_carry_sub_tail_def assign_var_carry_sub_nat_def
+          subtail_var_bit_to_var)
+  done
+
 
 lemma sub_assign_var_carry_sub: 
 "assign_var_carry_sub_nat i (vname_encode v) a b c = comm_encode(assign_var_carry_sub i v a b c)"
@@ -279,6 +424,23 @@ definition full_subtractor_nat:: "nat \<Rightarrow> nat \<Rightarrow> nat" where
                                                        (3 ## (op_b ## 0) ## (assign 0 0 1) ## ( assign 0 0 0) ## 0))##0)
 ## 0
  )"
+
+definition full_subtractor_tail:: "nat \<Rightarrow> nat \<Rightarrow> nat" where
+"full_subtractor_tail i v  = (let assign = assign_var_carry_sub_tail i v; op_a = operand_bit_to_var_tail (prod_encode(encode_char(CHR ''a''), i));
+  op_b = operand_bit_to_var_tail (prod_encode(encode_char (CHR ''b''), i)) in 
+3##(op_a ## 0) ##(3##((vname_encode ''carry'') ## 0)## (3 ## (op_b ## 0) ## (assign 1 1 1) ## ( assign 1 1 0) ## 0)##(
+                                                       (3 ## (op_b ## 0) ## (assign 1 0 1) ## ( assign 1 0 0) ## 0))##0)
+               ##(3##((vname_encode ''carry'') ## 0)## (3 ## (op_b ## 0) ## (assign 0 1 1) ## ( assign 0 1 0) ## 0)##(
+                                                       (3 ## (op_b ## 0) ## (assign 0 0 1) ## ( assign 0 0 0) ## 0))##0)
+## 0
+ )"
+
+lemma subtail_full_subtractor:
+"full_subtractor_tail i v = full_subtractor_nat i v"
+  apply(auto simp only: full_subtractor_tail_def full_subtractor_nat_def
+        subtail_assign_var_carry_sub subtail_operand_bit_to_var Let_def)
+  done
+
     
 lemma sub_full_subtractor: "full_subtractor_nat i (vname_encode v) = comm_encode (full_subtractor i v)"
   apply (auto simp only:full_subtractor_nat_def sub_assign_var_carry_sub
@@ -292,6 +454,17 @@ definition underflow_handler_nat:: "nat \<Rightarrow> nat \<Rightarrow> nat" whe
 binary_assign_constant_nat n v 0
 )##0)## (0##0) ## 0"
 
+definition underflow_handler_tail:: "nat \<Rightarrow> nat \<Rightarrow> nat" where
+"underflow_handler_tail n v = 3##((vname_encode ''carry'')## 0) ## (2##(1##(vname_encode ''carry'')##0##0)##(
+binary_assign_constant_tail n v 0
+)##0)## (0##0) ## 0"
+
+lemma subtail_underflow_handler:
+"underflow_handler_tail n v = underflow_handler_nat n v"
+  apply(auto simp only: underflow_handler_tail_def underflow_handler_nat_def
+subtail_binary_assign_constant
+) done
+
 lemma sub_underflow_handler:
  "underflow_handler_nat n (vname_encode v) = comm_encode (underflow_handler n v) "
   apply (auto simp only:underflow_handler_nat_def cons0 sub_cons underflow_handler_def
@@ -302,18 +475,77 @@ lemma sub_underflow_handler:
 fun map_full_subtractor :: "nat \<Rightarrow> nat \<Rightarrow> nat" where 
 "map_full_subtractor v n = (if n = 0 then 0 else (full_subtractor_nat(hd_nat n) v) ## map_full_subtractor v (tl_nat n))"
 
+
 lemma submap_full_subtractor: 
   "map_full_subtractor v n = map_nat (\<lambda>i. full_subtractor_nat i v) n"
   apply (induct v n rule : map_full_subtractor.induct)
   apply (subst map_full_subtractor.simps)
   apply (auto)
   done
-  
+
+fun map_full_subtractor_acc :: "nat \<Rightarrow> nat \<Rightarrow> nat \<Rightarrow> nat" where 
+"map_full_subtractor_acc acc v n = (if n =0 then acc else map_full_subtractor_acc ((full_subtractor_tail (hd_nat n) v)##acc)
+    v (tl_nat n)) "
+
+lemma map_full_subtractor_append:
+"map_full_subtractor v (append_nat xs ys) = append_nat (map_full_subtractor v xs) (map_full_subtractor v ys)"
+proof -
+  obtain xs' ys' where "xs= list_encode xs'" "ys = list_encode ys'"
+    by (metis list_decode_inverse)
+  thus ?thesis apply (auto simp add:sub_append submap_full_subtractor sub_map simp del:map_full_subtractor.simps 
+map_nat.simps) done
+qed
+
+lemma map_full_subtractor_induct: "
+reverse_nat (map_full_subtractor v (append_nat xs ys)) = 
+map_full_subtractor_acc (reverse_nat (map_full_subtractor v xs)) v ys
+  "
+  apply(induct ys arbitrary:xs rule:length_nat.induct)
+   apply(auto simp add: append_nat_0 append_nat_Suc  simp del: map_full_subtractor.simps map_full_subtractor_acc.simps)
+   apply simp
+  apply(subst (2) map_full_subtractor_acc.simps)
+  apply(auto simp add: map_full_subtractor_append 
+          reverse_append_nat subtail_full_subtractor  simp del: map_full_subtractor.simps map_full_subtractor_acc.simps)
+  apply(subst map_full_subtractor.simps)
+ apply(auto simp add:cons_Nil simp del:list_encode.simps map_full_subtractor.simps map_full_subtractor_acc.simps)
+  apply(auto simp add:cons0 sub_hd sub_tl 
+              simp del:list_encode.simps map_full_subtractor.simps map_full_subtractor_acc.simps)
+   apply(auto simp add: reverse_cons_nat 
+              simp del: map_full_subtractor.simps map_full_subtractor_acc.simps)  
+      apply(subst map_full_subtractor.simps)
+    apply(auto simp add: reverse_nat_0 append_singleton_nat
+              simp del: map_adder.simps map_adder_acc.simps)  
+  done
+
+definition map_full_subtractor_tail  where 
+"map_full_subtractor_tail v n = reverse_nat (map_full_subtractor_acc 0 v n) "
+
+lemma subtail_map_full_subtractor : 
+"map_full_subtractor_tail v n = map_full_subtractor v n"
+  using map_full_subtractor_induct[of v 0 n]  append_nat_0
+  apply (auto simp add: map_full_subtractor_tail_def simp  del: map_full_subtractor.simps map_full_subtractor_acc.simps)
+  using rev_rev_nat 
+  by (metis map_full_subtractor.simps reverse_nat_0)
+
 definition subtract_handle_underflow_nat:: 
   "nat \<Rightarrow> nat \<Rightarrow> nat" where
 "subtract_handle_underflow_nat n v = 2##
   (com_list_to_seq_nat (map_full_subtractor v (list_less_nat n)))## 
   (underflow_handler_nat n v) ## 0"
+
+definition subtract_handle_underflow_tail:: 
+  "nat \<Rightarrow> nat \<Rightarrow> nat" where
+"subtract_handle_underflow_tail n v = 2##
+  (com_list_to_seq_tail (map_full_subtractor_tail v (list_less_tail n)))## 
+  (underflow_handler_tail n v) ## 0"
+
+lemma subtail_subtract_handle_underflow:
+" subtract_handle_underflow_tail n v =  subtract_handle_underflow_nat n v"
+  apply( auto simp only: subtract_handle_underflow_tail_def 
+          subtract_handle_underflow_nat_def 
+          subtail_com_list_to_seq subtail_map_full_subtractor subtail_list_less 
+            subtail_underflow_handler)
+  done
 
 lemma sub_subtract_underflow : 
 "subtract_handle_underflow_nat n (vname_encode v) = comm_encode ( subtract_handle_underflow n v)"
@@ -336,6 +568,23 @@ definition binary_subtractor_nat:: "nat \<Rightarrow> nat \<Rightarrow> nat \<Ri
 ) ## 0
 ) ## 0"
 
+definition binary_subtractor_tail:: "nat \<Rightarrow> nat \<Rightarrow> nat \<Rightarrow> nat \<Rightarrow>nat" where
+"binary_subtractor_tail n v a b = 
+2 ## (copy_atom_to_operand_tail n (encode_char(CHR ''a'')) a) ## (
+2 ## (   copy_atom_to_operand_tail n (encode_char(CHR ''b'')) b) ## (
+2 ## (subtract_handle_underflow_tail n v) ##(
+2##(copy_atom_to_operand_tail n (encode_char(CHR ''a'')) (prod_encode(1,0)))##(
+  copy_atom_to_operand_tail n (encode_char(CHR ''b'')) (prod_encode(1,0)))##0 
+) ## 0
+) ## 0
+) ## 0"
+
+lemma subtail_binary_subtractor: 
+"binary_subtractor_tail n v a b = binary_subtractor_nat n v a b  "
+  apply(auto simp only: binary_subtractor_tail_def binary_subtractor_nat_def
+        subtail_copy_atom_to_operand subtail_subtract_handle_underflow)
+  done
+
 lemma sub_binary_subtractor:
 "binary_subtractor_nat n (vname_encode v) (atomExp_encode a) (atomExp_encode b) =
     comm_encode (binary_subtractor n v a b)"
@@ -352,6 +601,22 @@ else 2## (3 ## ((var_bit_to_var_nat(prod_encode(snd_nat a, 0))) ## 0) ## (binary
 2 ## (copy_atom_to_operand_nat n (encode_char (CHR ''a'')) a) ##
  (copy_atom_to_operand_nat n (encode_char (CHR ''a'')) (prod_encode(1,0))) ## 0
 ) ## 0 )"
+
+definition binary_parity_tail:: "nat \<Rightarrow> nat \<Rightarrow> nat \<Rightarrow> nat" where
+"binary_parity_tail n v a  = (if fst_nat a \<noteq> 0 then  binary_assign_constant_tail n v (snd_nat a mod 2)
+else 2## (3 ## ((var_bit_to_var_tail(prod_encode(snd_nat a, 0))) ## 0) ## (binary_assign_constant_tail n v 1) 
+ ##( binary_assign_constant_tail n v 0) ## 0)## (
+2 ## (copy_atom_to_operand_tail n (encode_char (CHR ''a'')) a) ##
+ (copy_atom_to_operand_tail n (encode_char (CHR ''a'')) (prod_encode(1,0))) ## 0
+) ## 0 )"
+
+
+lemma subtail_binary_parity:
+"binary_parity_tail n v a = binary_parity_nat n v a"
+  apply(auto simp only: binary_parity_tail_def binary_parity_nat_def
+              subtail_var_bit_to_var subtail_binary_assign_constant
+               subtail_copy_atom_to_operand)
+  done
 
 lemma sub_binary_parity:
  "binary_parity_nat n (vname_encode v) (atomExp_encode a) = comm_encode(binary_parity n v a) "
@@ -378,6 +643,42 @@ assign_shifted_bits_nat (i-1) v
 )##0
 )" 
 
+fun assign_shifted_bits_acc:: "nat \<Rightarrow> nat \<Rightarrow> nat \<Rightarrow> nat \<Rightarrow> nat" where
+"assign_shifted_bits_acc acc diff i v = (if diff  = 0 then acc else assign_shifted_bits_acc (
+2##( 
+3##((operand_bit_to_var_tail (prod_encode (encode_char(CHR ''a''), i-diff +1 )))##0)##(
+1## (var_bit_to_var_tail (prod_encode(v, i-diff)))## 1 ##0)##(
+1## (var_bit_to_var_tail (prod_encode(v, i-diff)))## 0 ##0
+)##0)## (
+acc
+)##0) (diff-1) i v
+)"
+
+lemma assign_shifted_bits_induct:
+"diff \<le> i \<Longrightarrow>assign_shifted_bits_acc (assign_shifted_bits_nat (i-diff) v) diff i v = 
+assign_shifted_bits_nat i v"
+  apply(induct diff)
+   apply simp
+  apply(subst assign_shifted_bits_acc.simps)
+  apply(auto simp add: subtail_operand_bit_to_var 
+subtail_var_bit_to_var
+simp del: assign_shifted_bits_acc.simps assign_shifted_bits_nat.simps operand_bit_to_var_nat.simps)
+  apply(subst (asm) assign_shifted_bits_nat.simps)
+ apply(auto simp add:
+simp del: assign_shifted_bits_acc.simps assign_shifted_bits_nat.simps operand_bit_to_var_nat.simps)
+  using Suc_diff_Suc Suc_le_lessD apply presburger
+  done
+
+definition assign_shifted_bits_tail :: "nat \<Rightarrow> nat \<Rightarrow> nat" where 
+"assign_shifted_bits_tail i v = assign_shifted_bits_acc (0##0) i i v"
+
+lemma subtail_assign_shifted_bits:
+"assign_shifted_bits_tail i v =assign_shifted_bits_nat i v "
+  apply(auto simp only: assign_shifted_bits_tail_def)
+  using assign_shifted_bits_induct[of i i v]
+  apply auto
+  done
+
 lemma sub_assign_shifted_bits:
 "assign_shifted_bits_nat i (vname_encode v) = comm_encode (assign_shifted_bits i v)"
   apply (induct i)
@@ -397,6 +698,18 @@ definition assign_shifted_bits_and_zero_most_significant_nat::
 "assign_shifted_bits_and_zero_most_significant_nat n v = 2 ## (assign_shifted_bits_nat (n - 1) v)##
   (1 ## (var_bit_to_var_nat (prod_encode(v, n - 1)))##0##0) ## 0"
 
+definition assign_shifted_bits_and_zero_most_significant_tail:: 
+  "nat \<Rightarrow> nat \<Rightarrow> nat" where
+"assign_shifted_bits_and_zero_most_significant_tail n v = 2 ## (assign_shifted_bits_tail (n - 1) v)##
+  (1 ## (var_bit_to_var_tail (prod_encode(v, n - 1)))##0##0) ## 0"
+
+lemma subtail_assign_shifted_bits_and_zero_most_significant:
+" assign_shifted_bits_and_zero_most_significant_tail n v =  assign_shifted_bits_and_zero_most_significant_nat n v "
+  apply(auto simp only:  assign_shifted_bits_and_zero_most_significant_nat_def 
+ assign_shifted_bits_and_zero_most_significant_tail_def
+  subtail_var_bit_to_var subtail_assign_shifted_bits)
+  done
+
 lemma sub_assign_shifted_bits_and_zero_most_significant:
 " assign_shifted_bits_and_zero_most_significant_nat n (vname_encode v) =
   comm_encode (assign_shifted_bits_and_zero_most_significant n v)"
@@ -411,6 +724,17 @@ definition binary_right_shift_nat:: "nat \<Rightarrow> nat \<Rightarrow> nat \<R
 "binary_right_shift_nat n v a = 2 ## (2 ## (copy_atom_to_operand_nat n (encode_char(CHR ''a'')) a) ##
 (assign_shifted_bits_and_zero_most_significant_nat n v) ## 0) ##
     (copy_atom_to_operand_nat n (encode_char(CHR ''a'')) (prod_encode(1,0))) ## 0" 
+
+definition binary_right_shift_tail:: "nat \<Rightarrow> nat \<Rightarrow> nat \<Rightarrow> nat" where
+"binary_right_shift_tail n v a = 2 ## (2 ## (copy_atom_to_operand_tail n (encode_char(CHR ''a'')) a) ##
+(assign_shifted_bits_and_zero_most_significant_tail n v) ## 0) ##
+    (copy_atom_to_operand_tail n (encode_char(CHR ''a'')) (prod_encode(1,0))) ## 0" 
+
+lemma subtail_binary_right_shift:
+"binary_right_shift_tail n v a = binary_right_shift_nat n v a"
+  apply(auto simp only: binary_right_shift_tail_def  binary_right_shift_nat_def
+   subtail_copy_atom_to_operand subtail_assign_shifted_bits_and_zero_most_significant
+  )done
 
 lemma sub_binary_right_shift:
   "binary_right_shift_nat n (vname_encode v) (atomExp_encode a) = comm_encode (binary_right_shift n v a)"
@@ -429,6 +753,21 @@ else if hd_nat aexp = 2 then binary_subtractor_nat n v (nth_nat (Suc 0) aexp) (n
 else if hd_nat aexp = 3 then binary_parity_nat n v (nth_nat (Suc 0) aexp)
 else  binary_right_shift_nat n v (nth_nat (Suc 0) aexp)
 )"
+
+definition assignment_to_binary_tail:: "nat \<Rightarrow> nat \<Rightarrow>nat \<Rightarrow> nat" where
+"assignment_to_binary_tail n v aexp = (if hd_nat aexp =0 then 
+   binary_adder_tail n v (nth_nat (Suc 0) aexp) (prod_encode (1,0))
+else if hd_nat aexp = 1 then binary_adder_tail n v (nth_nat (Suc 0) aexp) (nth_nat (Suc (Suc 0)) aexp)
+else if hd_nat aexp = 2 then binary_subtractor_tail n v (nth_nat (Suc 0) aexp) (nth_nat (Suc (Suc 0)) aexp)
+else if hd_nat aexp = 3 then binary_parity_tail n v (nth_nat (Suc 0) aexp)
+else  binary_right_shift_tail n v (nth_nat (Suc 0) aexp)
+)"
+
+lemma subtail_assignment_to_binary :
+ "assignment_to_binary_tail n v aexp = assignment_to_binary_nat n v aexp"
+  apply(auto simp only: assignment_to_binary_tail_def assignment_to_binary_nat_def
+    subtail_binary_adder subtail_binary_subtractor subtail_binary_right_shift subtail_binary_parity
+) done
 
 lemma sub_assignment_to_binary:
 "assignment_to_binary_nat n (vname_encode v) (aexp_encode aexp) = 
