Cook_Levin/IMP-_To_SAS+/IMP-_To_IMP--/IMP_Minus_To_IMP_Minus_Minus_nat.thy
@@ -6,14 +6,74 @@ begin
 fun map_var_bit_to_var:: "nat \<Rightarrow> nat \<Rightarrow> nat" where 
 "map_var_bit_to_var v n = (if n =0 then 0 else (var_bit_to_var_nat (prod_encode (v,hd_nat n)))## map_var_bit_to_var v (tl_nat n)  )"
 
+fun map_var_bit_to_var_acc :: "nat \<Rightarrow> nat \<Rightarrow> nat \<Rightarrow> nat" where 
+"map_var_bit_to_var_acc acc v n = (if n =0 then acc 
+else map_var_bit_to_var_acc ((var_bit_to_var_tail (prod_encode (v,hd_nat n)))## acc) v (tl_nat n)  )"
+
 lemma submap_var_bit_to_var :
 "map_var_bit_to_var v n =  map_nat (\<lambda>i. var_bit_to_var_nat (prod_encode (v,i))) n "
   apply (induct v n rule:map_var_bit_to_var.induct)
   apply auto
   done
 
+
+lemma map_var_bit_to_var_append:
+"map_var_bit_to_var v (append_nat xs ys) = 
+append_nat(map_var_bit_to_var v xs) (map_var_bit_to_var v ys)"
+proof -
+  obtain xs' ys' where "ys = list_encode ys'"  "xs = list_encode xs'" 
+  by (metis list_decode_inverse)
+  thus ?thesis 
+    apply(auto simp add: sub_append submap_var_bit_to_var
+sub_map
+ simp del:map_nat.simps
+map_var_bit_to_var.simps)
+    done
+qed
+
+lemma map_var_bit_to_var_induct:
+"reverse_nat (map_var_bit_to_var v (append_nat xs ys))
+= map_var_bit_to_var_acc (reverse_nat (map_var_bit_to_var v xs)) v ys"
+  apply(induct ys arbitrary:xs rule:length_nat.induct)
+   apply(auto simp del:  map_var_bit_to_var_acc.simps  map_var_bit_to_var.simps
+          simp add: append_nat_0)
+   apply simp
+    apply(auto simp del:  map_var_bit_to_var_acc.simps  map_var_bit_to_var.simps
+          simp add: append_nat_0 append_nat_Suc)
+  apply (subst (2) map_var_bit_to_var_acc.simps)
+  apply(auto simp add: map_var_bit_to_var_append subtail_var_bit_to_var
+        reverse_append_nat simp del:  map_var_bit_to_var_acc.simps  map_var_bit_to_var.simps
+          simp add: append_nat_0 append_nat_Suc)
+  apply(subst map_var_bit_to_var.simps)
+  apply(auto simp add: cons_Nil
+ simp del:  map_var_bit_to_var_acc.simps  map_var_bit_to_var.simps)
+
+  apply(auto simp only: cons0 sub_hd head.simps sub_tl tail.simps)
+  apply(subst map_var_bit_to_var.simps)
+    apply(auto simp add: reverse_singleton_nat append_singleton_nat
+ simp del:  map_var_bit_to_var_acc.simps  map_var_bit_to_var.simps)
+  done
+
+definition map_var_bit_to_var_tail :: "nat \<Rightarrow> nat \<Rightarrow> nat" where 
+"map_var_bit_to_var_tail v n = reverse_nat (map_var_bit_to_var_acc 0 v n)"
+
+lemma subtail_map_var_bit_to_var:
+"map_var_bit_to_var_tail v n = map_var_bit_to_var v n"
+  apply(auto simp only: map_var_bit_to_var_tail_def)
+  using map_var_bit_to_var_induct [of v 0 n] rev_rev_nat map_var_bit_to_var.simps
+  by (metis append_nat.simps(1) reverse_nat_0)
+
 definition var_bit_list_nat :: "nat \<Rightarrow> nat \<Rightarrow> nat" where 
 "var_bit_list_nat n v = map_var_bit_to_var v (list_less_nat n)"
+
+definition var_bit_list_tail :: "nat \<Rightarrow> nat \<Rightarrow> nat" where 
+"var_bit_list_tail n v = map_var_bit_to_var_tail v (list_less_tail n)"
+
+lemma subtail_var_bit_list: 
+"var_bit_list_tail n v = var_bit_list_nat n v"
+  apply(auto simp only: var_bit_list_tail_def var_bit_list_nat_def 
+          subtail_list_less subtail_map_var_bit_to_var)
+  done
 
 lemma sub_var_bit_list: "var_bit_list_nat n (vname_encode v) = vname_list_encode (var_bit_list n v)"
   apply (simp only: submap_var_bit_to_var  var_bit_list_nat_def var_bit_list_def sub_var_bit_to_var sub_map sub_list_less
@@ -24,6 +84,38 @@ lemma sub_var_bit_list: "var_bit_list_nat n (vname_encode v) = vname_list_encode
 
 
 declare nth_nat.simps[simp del]
+datatype IMPm_IMPmm = SKIP | 
+                      Assign vname aexp |
+                      Seq_0 IMP_Minus_com IMP_Minus_com |
+                      Seq_m IMP_Minus_com IMP_Minus_com IMP_Minus_Minus_com |
+                      Seq_f IMP_Minus_com IMP_Minus_com IMP_Minus_Minus_com IMP_Minus_Minus_com |
+                      If_0  vname IMP_Minus_com IMP_Minus_com |
+                      If_m  vname IMP_Minus_com IMP_Minus_com IMP_Minus_Minus_com |
+                      If_f vname IMP_Minus_com IMP_Minus_com IMP_Minus_Minus_com IMP_Minus_Minus_com |
+                      While_0 vname IMP_Minus_com|
+                      While_f vname IMP_Minus_com IMP_Minus_Minus_com
+
+fun push_on_Stack :: "IMP_Minus_com \<Rightarrow> IMPm_IMPmm list \<Rightarrow> IMPm_IMPmm list" where 
+"push_on_Stack Com.SKIP stack = SKIP # stack "|
+"push_on_Stack (Com.Assign v aexp) stack =  ( Assign v aexp) # stack "|
+"push_on_Stack (Com.Seq c1 c2) stack =  ( Seq_0 c1 c2) # stack "|
+"push_on_Stack (Com.If v c1 c2) stack =  (If_0 v c1 c2) # stack "|
+"push_on_Stack (Com.While v c) stack =  (While_0 v c) # stack "
+
+fun add_result_to_stack :: "IMP_Minus_Minus_com \<Rightarrow> IMPm_IMPmm list \<Rightarrow> IMPm_IMPmm list" where 
+"add_result_to_stack"
+
+                      
+fun IMP_Minus_To_IMP_Minus_Minus:: "IMP_Minus_com \<Rightarrow> nat \<Rightarrow> IMP_Minus_Minus_com" where
+"IMP_Minus_To_IMP_Minus_Minus Com.SKIP n = IMP_Minus_Minus_Com.SKIP" |
+"IMP_Minus_To_IMP_Minus_Minus (Com.Assign v aexp) n = assignment_to_binary n v aexp" |
+"IMP_Minus_To_IMP_Minus_Minus (Com.Seq c1 c2) n = 
+  (IMP_Minus_To_IMP_Minus_Minus c1 n ;; IMP_Minus_To_IMP_Minus_Minus c2 n )" |
+"IMP_Minus_To_IMP_Minus_Minus (Com.If v c1 c2) n = (IF (var_bit_list n v)\<noteq>0 THEN
+  IMP_Minus_To_IMP_Minus_Minus c1 n ELSE IMP_Minus_To_IMP_Minus_Minus c2 n)" |
+"IMP_Minus_To_IMP_Minus_Minus (Com.While v c) n = (WHILE (var_bit_list n v)\<noteq>0 DO
+  IMP_Minus_To_IMP_Minus_Minus c n)"
+
 fun IMP_Minus_To_IMP_Minus_Minus_nat:: "nat \<Rightarrow> nat \<Rightarrow> nat" where
 "IMP_Minus_To_IMP_Minus_Minus_nat c n = (if c =0 \<or> hd_nat c = 0 then  0##0
 else if hd_nat c = 1 then assignment_to_binary_nat n (nth_nat (Suc 0) c) (nth_nat (Suc (Suc 0)) c)
@@ -34,6 +126,7 @@ else if hd_nat c = 3 then
 else 
 4 ## (var_bit_list_nat n (nth_nat (Suc 0) c)) ## (IMP_Minus_To_IMP_Minus_Minus_nat (nth_nat (Suc(Suc 0)) c) n) ## 0
 )"
+
 declare nth_nat.simps[simp]
 
 lemma sub_IMP_Minus_To_IMP_Minus_Minus:
